feat: (5.2) specify constructor and valid

Project 1/Ex5.dfy
@@ -4,17 +4,53 @@ module Ex5 {
   
   import Ex3=Ex3
 
+  function allFalse(tbl : array<bool>) : bool
+  {
+    forall i :: 0 <= i < tbl.Length ==> !tbl[i]
+  }
+
   class Set {
     var tbl : array<bool>  
     var list : Ex3.Node?
 
-    ghost function Valid() : bool 
-    {
+    ghost var content : set<nat>
+    ghost var footprint : set<Ex3.Node>
 
+    ghost function Valid() : bool
+      reads this, this.footprint, this.list, this.tbl
+    {
+      if (this.list == null)
+        then 
+          this.footprint == {}
+          &&
+          this.content == {}
+          &&
+          allFalse(this.tbl)
+        else 
+          this.footprint == this.list.footprint
+          &&
+          this.content == this.list.content
+          &&
+          this.list.val in this.content
+          &&
+          0 <= this.list.val < this.tbl.Length
+          &&
+          tbl[this.list.val]
+          &&
+          this.list.Valid()
     }
       
-    constructor (size : nat) 
+    constructor (size : nat)
+      ensures Valid()
+      ensures this.tbl.Length == size && forall i :: 0 <= i < size ==> !this.tbl[i]
+      ensures this.list == null
+      ensures this.content == {} && this.footprint == {}
     {
+      tbl := new bool[size](x => false);
+      list := null;
+
+      content := {};
+      footprint := {};
     }
 
 
